

Boolean Algebra: Group Exercises

CSCI 246

January 28, 2026

Problem 1. For each property, give an equation showing the property.

Example. *Commutative property \wedge :* $x \wedge y = y \wedge x$.

A. *Commutative property \vee :* $x \vee y = y \vee x$.

B. *Associativity \wedge :* $x \wedge (y \wedge z) = (x \wedge y) \wedge z$.

C. *Associativity \vee :* $x \vee (y \vee z) = (x \vee y) \vee z$.

D. *Identity element \wedge :* $1 \wedge x = x \wedge 1 = x$.

E. *Identity element \vee :* $0 \vee x = x \vee 0 = x$.

F. *Double negation:* $\neg\neg x = x$.

G. *DeMorgan's Law:* $\neg(x \wedge y) = \neg x \vee \neg y$ and $\neg(x \vee y) = \neg x \wedge \neg y$.

H. *Idempotency \vee :* $x \vee x = x$.

I. *Idempotency \wedge :* $x \wedge x = x$.

J. *Distributivity:* $(x \wedge y) \vee z = (x \vee z) \wedge (y \vee z)$ and $(x \vee y) \wedge z = (x \wedge z) \vee (y \wedge z)$.

K. *Law of excluded middle:* $x \vee \neg x = 1$

L. *Complement law:* $x \wedge \neg x = 0$.

Problem 2. Show that $a \implies b$ is equivalent to $(\neg a) \vee b$.

a	b	$a \implies b$	$\neg a \vee b$
0	0	1	1
0	1	1	1
1	0	0	0
1	1	1	1

Problem 3. Prove that $(x \wedge y) \vee (x \wedge \neg y)$ is equivalent to x .

x	y	$(\mathbf{x} \wedge \mathbf{y}) \vee (\mathbf{x} \wedge \neg \mathbf{y})$
0	0	0
0	1	0
1	0	1
1	1	1

Alternatively, you can use the rules from Problem 1 to prove the equivalence.

$$(x \wedge y) \vee (x \wedge \neg y)$$

By distributivity of \vee and \wedge we can foil the expression to:

$$(x \vee x) \wedge (x \vee \neg y) \wedge (y \vee x) \wedge (y \vee \neg y)$$

We can then simplify using idempotency of \vee and law of excluded middle:

$$x \wedge (x \vee \neg y) \wedge (y \vee x) \wedge 1$$

Further simplify by multiplication identity, commutativity, and distributivity:

$$x \wedge (x \vee (\neg y \wedge y))$$

We next use the complement law and simplify using disjunctive identity:

$$x \wedge x$$

Finally, we simplify using idempotency of \wedge :

$$x$$

Problem 4. Show that the following are *tautologies*.

A. $(x \vee y) \implies (x \vee (y \wedge z)) \vee (x \vee \neg z)$.

x	y	z	$(x \vee y) \implies (x \vee (y \wedge z)) \vee (x \vee \neg z)$
0	0	0	1
0	0	1	1
0	1	0	1
0	1	1	1
1	0	0	1
1	0	1	1
1	1	0	1
1	1	1	1

B. $(x \wedge (y \implies z)) \implies ((x \wedge y) \implies (x \wedge z))$.

x	y	z	$(x \wedge (y \implies z)) \implies ((x \wedge y) \implies (x \wedge z))$
0	0	0	1
0	0	1	1
0	1	0	1
0	1	1	1
1	0	0	1
1	0	1	1
1	1	0	1
1	1	1	1

C. $(x \vee y) \wedge (\neg x \vee z) \implies (y \vee z)$.

x	y	z	$(x \vee y) \wedge (\neg x \vee z) \implies (y \vee z)$
0	0	0	1
0	0	1	1
0	1	0	1
0	1	1	1
1	0	0	1
1	0	1	1
1	1	0	1
1	1	1	1

D. $x \vee (\neg x \wedge (x \vee y)) \vee \neg y$.

x	y	$x \vee (\neg x \wedge (x \vee y)) \vee \neg y$
0	0	1
0	1	1
1	0	1
1	1	1